halfway through verifying generate funciton

specs/HMAC256_DRBG_functional_prog.v
@@ -15,7 +15,7 @@ Definition HMAC256_DRBG_instantiate_algorithm := HMAC_DRBG_instantiate_algorithm
 
 Definition HMAC256_DRBG_instantiate_function := DRBG_instantiate_function HMAC256_DRBG_instantiate_algorithm.
 
-Definition HMAC256_DRBG_generate_algorithm := HMAC_DRBG_generate_algorithm HMAC256 1024.
+Definition HMAC256_DRBG_generate_algorithm := HMAC_DRBG_generate_algorithm HMAC256.
 
 Definition HMAC256_DRBG_generate_function := DRBG_generate_function HMAC256_DRBG_generate_algorithm.
 
