specs/verif_hmac_drbg_generate.v
@@ -1,0 +1,461 @@
+Require Import floyd.proofauto.
+Import ListNotations.
+Local Open Scope logic.
+
+Require Import sha.HMAC256_functional_prog.
+Require Import sha.general_lemmas.
+Require Import sha.spec_sha.
+
+Require Import HMAC256_DRBG_functional_prog.
+Require Import HMAC_DRBG_generate_algorithm.
+Require Import hmac_drbg.
+Require Import spec_hmac_drbg.
+Require Import DRBG_generate_function.
+Require Import entropy.
+
+Lemma body_hmac_drbg_reseed: semax_body HmacDrbgVarSpecs HmacDrbgFunSpecs 
+       f_mbedtls_hmac_drbg_random_with_add hmac_drbg_generate_spec.
+Proof.
+  start_function.
+
+  name p_rng' _p_rng.
+  name ctx' _ctx.
+  name add_len' _len.
+  name additional' _additional.
+  name out_len' _out_len.
+  name output' _output.
+  name out' _out.
+  
+  destruct initial_state_abs.
+  destruct initial_state as [md_ctx' [V' [reseed_counter' [entropy_len' [prediction_resistance' reseed_interval']]]]].
+  unfold hmac256drbg_relate.
+  normalize.
+  
+  (* mbedtls_hmac_drbg_context *ctx = p_rng; *)
+  forward.
+  assert_PROP (ctx = (force_val (sem_cast_neutral ctx))) as Hctx by entailer!.
+  rewrite <- Hctx; clear Hctx.
+
+  (* int left = out_len *)
+  forward.
+
+  (* out = output *)
+  forward.
+
+  (* prediction_resistance = ctx->prediction_resistance *)
+  forward.
+  {
+    (* typechecking *)
+    entailer!.
+    destruct prediction_resistance; constructor.
+  }
+
+  (* reseed_counter = ctx->reseed_counter *)
+  forward.
+
+  (* reseed_interval = ctx->reseed_interval *)
+  forward.
+
+  (* info = ctx->md_ctx.md_info; *)
+  forward.
+
+  (* md_len = mbedtls_md_get_size(info); *)
+  forward_call tt.
+  Intros md_len.
+
+  (* if( out_len > MBEDTLS_HMAC_DRBG_MAX_REQUEST ) *)
+  forward_if (PROP  (out_len <= 1024)
+      LOCAL  (temp _md_len md_len; temp _info (let (x, _) := md_ctx' in x);
+      temp _reseed_interval (Vint (Int.repr reseed_interval));
+      temp _reseed_counter (Vint (Int.repr reseed_counter));
+      temp _prediction_resistance (Val.of_bool prediction_resistance);
+      temp _out output; temp _left (Vint (Int.repr out_len)); 
+      temp _ctx ctx; temp _p_rng ctx; temp _output output;
+      temp _out_len (Vint (Int.repr out_len)); temp _additional additional;
+      temp _add_len (Vint (Int.repr add_len)); gvar sha._K256 kv)
+      SEP  (memory_block Tsh out_len output;
+      data_at Tsh (tarray tuchar add_len) (map Vint (map Int.repr contents))
+        additional;
+      data_at Tsh t_struct_hmac256drbg_context_st
+        (md_ctx',
+        (map Vint (map Int.repr V),
+        (Vint (Int.repr reseed_counter),
+        (Vint (Int.repr entropy_len),
+        (Val.of_bool prediction_resistance, Vint (Int.repr reseed_interval))))))
+        ctx; md_full md_ctx md_ctx';
+      data_at Tsh t_struct_mbedtls_md_info info_contents
+        (hmac256drbgstate_md_info_pointer
+           (md_ctx',
+           (map Vint (map Int.repr V),
+           (Vint (Int.repr reseed_counter),
+           (Vint (Int.repr entropy_len),
+           (Val.of_bool prediction_resistance,
+           Vint (Int.repr reseed_interval))))))); Stream s;
+      spec_sha.K_vector kv)).
+  {
+    (* return( MBEDTLS_ERR_HMAC_DRBG_REQUEST_TOO_BIG ); *)
+    forward.
+
+    (* prove post condition of the function *)
+    unfold hmac_drbg_update_post, get_stream_result, hmac256drbg_relate.
+    Exists (HMAC256DRBGabs md_ctx V reseed_counter entropy_len prediction_resistance reseed_interval) (Vint (Int.repr (-3))) (md_ctx',
+        (map Vint (map Int.repr V),
+        (Vint (Int.repr reseed_counter),
+        (Vint (Int.repr entropy_len),
+        (Val.of_bool prediction_resistance, Vint (Int.repr reseed_interval)))))).
+    destruct md_ctx.
+    rewrite andb_negb_r.
+    assert (Hout_len: out_len >? 1024 = true).
+    {
+      rewrite Z.gtb_ltb.
+      apply Z.ltb_lt.
+      assumption.
+    }
+    rewrite Hout_len.
+    entailer!.
+  }
+  {
+    forward.
+    entailer!.
+  }
+
+  normalize.
+  assert (Hout_len: 0 <= out_len <= 1024) by omega.
+  assert (Hout_lenb: out_len >? 1024 = false).
+  {
+    rewrite Z.gtb_ltb.
+    apply Z.ltb_nlt.
+    omega.
+  }
+
+  (* if( add_len > MBEDTLS_HMAC_DRBG_MAX_INPUT ) *)
+  forward_if (PROP  (add_len <= 256)
+      LOCAL  (temp _md_len md_len; temp _info (let (x, _) := md_ctx' in x);
+      temp _reseed_interval (Vint (Int.repr reseed_interval));
+      temp _reseed_counter (Vint (Int.repr reseed_counter));
+      temp _prediction_resistance (Val.of_bool prediction_resistance);
+      temp _out output; temp _left (Vint (Int.repr out_len)); 
+      temp _ctx ctx; temp _p_rng ctx; temp _output output;
+      temp _out_len (Vint (Int.repr out_len)); temp _additional additional;
+      temp _add_len (Vint (Int.repr add_len)); gvar sha._K256 kv)
+      SEP  (memory_block Tsh out_len output;
+      data_at Tsh (tarray tuchar add_len) (map Vint (map Int.repr contents))
+        additional;
+      data_at Tsh t_struct_hmac256drbg_context_st
+        (md_ctx',
+        (map Vint (map Int.repr V),
+        (Vint (Int.repr reseed_counter),
+        (Vint (Int.repr entropy_len),
+        (Val.of_bool prediction_resistance, Vint (Int.repr reseed_interval))))))
+        ctx; md_full md_ctx md_ctx';
+      data_at Tsh t_struct_mbedtls_md_info info_contents
+        (hmac256drbgstate_md_info_pointer
+           (md_ctx',
+           (map Vint (map Int.repr V),
+           (Vint (Int.repr reseed_counter),
+           (Vint (Int.repr entropy_len),
+           (Val.of_bool prediction_resistance,
+           Vint (Int.repr reseed_interval))))))); Stream s;
+      spec_sha.K_vector kv)).
+  {
+    (* return( MBEDTLS_ERR_HMAC_DRBG_INPUT_TOO_BIG ); *)
+    forward.
+
+    (* prove function post condition *)
+    unfold hmac_drbg_update_post, get_stream_result, hmac256drbg_relate.
+    Exists (HMAC256DRBGabs md_ctx V reseed_counter entropy_len prediction_resistance reseed_interval) (Vint (Int.repr (-5))) (md_ctx',
+        (map Vint (map Int.repr V),
+        (Vint (Int.repr reseed_counter),
+        (Vint (Int.repr entropy_len),
+        (Val.of_bool prediction_resistance, Vint (Int.repr reseed_interval)))))).
+    destruct md_ctx.
+    rewrite andb_negb_r.
+    rewrite Hout_lenb.
+    assert (Hlength_contents: Zlength contents >? 256 = true).
+    {
+      rewrite Z.gtb_ltb.
+      apply Z.ltb_lt.
+      assumption.
+    }
+    replace (Z.of_nat (length contents)) with (Zlength contents) by (rewrite Zlength_correct; auto).
+    rewrite Hlength_contents.
+    entailer!.
+  }
+  {
+    forward.
+    entailer!.
+  }
+  normalize.
+  assert (Hadd_len: 0 <= add_len <= 256) by omega.
+  assert (Hadd_lenb: add_len >? 256 = false).
+  {
+    rewrite Z.gtb_ltb.
+    apply Z.ltb_nlt.
+    omega.
+  }
+  remember (orb prediction_resistance (reseed_counter >? reseed_interval)) as should_reseed.
+  forward_if (PROP  ()
+      LOCAL  (temp _md_len md_len; temp _info (let (x, _) := md_ctx' in x);
+      temp _reseed_interval (Vint (Int.repr reseed_interval));
+      temp _reseed_counter (Vint (Int.repr reseed_counter));
+      temp _prediction_resistance (Val.of_bool prediction_resistance);
+      temp _out output; temp _left (Vint (Int.repr out_len)); 
+      temp _ctx ctx; temp _p_rng ctx; temp _output output;
+      temp _out_len (Vint (Int.repr out_len)); temp _additional additional;
+      temp _add_len (Vint (Int.repr add_len)); gvar sha._K256 kv;
+      temp 159%positive (Val.of_bool should_reseed)
+             )
+      SEP  (memory_block Tsh out_len output;
+      data_at Tsh (tarray tuchar add_len) (map Vint (map Int.repr contents))
+        additional;
+      data_at Tsh t_struct_hmac256drbg_context_st
+        (md_ctx',
+        (map Vint (map Int.repr V),
+        (Vint (Int.repr reseed_counter),
+        (Vint (Int.repr entropy_len),
+        (Val.of_bool prediction_resistance, Vint (Int.repr reseed_interval))))))
+        ctx; md_full md_ctx md_ctx';
+      data_at Tsh t_struct_mbedtls_md_info info_contents
+        (hmac256drbgstate_md_info_pointer
+           (md_ctx',
+           (map Vint (map Int.repr V),
+           (Vint (Int.repr reseed_counter),
+           (Vint (Int.repr entropy_len),
+           (Val.of_bool prediction_resistance,
+           Vint (Int.repr reseed_interval))))))); Stream s;
+      spec_sha.K_vector kv)).
+  {
+    forward.
+    entailer!.
+    
+    rename H10 into Hpr.
+    destruct prediction_resistance.
+    (* true *) reflexivity.
+    (* false *)
+    inversion Hpr.
+  }
+  {
+    rename H10 into Hpr.
+    destruct prediction_resistance; try solve [inversion Hpr].
+    simpl in Heqshould_reseed.
+    forward.
+    subst should_reseed.
+    entailer!.
+    rewrite <- H11.
+    
+    rewrite Z.gtb_ltb.
+    unfold Int.lt.
+    destruct (zlt reseed_interval reseed_counter) as [Hlt | Hlt].
+    {
+      (* reseed_interval < reseed_counter *)
+      assert (Hltb: reseed_interval <? reseed_counter = true) by (rewrite Z.ltb_lt; assumption).
+      rewrite Hltb.
+      (* TODO *) admit.
+    }
+    {
+      assert (Hltb: reseed_interval <? reseed_counter = false) by (rewrite Z.ltb_nlt; assumption).
+      rewrite Hltb.
+      (* TODO *) admit.
+    }
+  }
+  unfold hmac256drbgstate_md_info_pointer.
+  simpl.
+  forward_if (
+      PROP  (
+      )
+      LOCAL  (temp _md_len md_len; temp _info (let (x, _) := md_ctx' in x);
+      temp _reseed_interval (Vint (Int.repr reseed_interval));
+      temp _reseed_counter (Vint (Int.repr reseed_counter));
+      temp _prediction_resistance (Val.of_bool prediction_resistance);
+      temp _out output; temp _left (Vint (Int.repr out_len)); 
+      temp _ctx ctx; temp _p_rng ctx; temp _output output;
+      temp _out_len (Vint (Int.repr out_len)); temp _additional additional;
+      temp _add_len (Vint (Int.repr (if should_reseed then 0 else add_len))); gvar sha._K256 kv;
+      temp 159%positive (Val.of_bool should_reseed))
+      SEP  (
+        if should_reseed then
+          match (mbedtls_HMAC256_DRBG_reseed_function s (HMAC256DRBGabs md_ctx V reseed_counter entropy_len prediction_resistance reseed_interval) contents) with
+            | ENTROPY.error _ s' => !!False (* bogus, not used since the function returns *)
+            | ENTROPY.success state_handle s' =>
+              EX data:_,
+              let state_abs := (hmac256drbgabs_convert_state_handle state_handle data entropy_len reseed_interval) in
+              !!(Zlength (hmac256drbgabs_value state_abs) = Z.of_nat SHA256.DigestLength
+                 /\ Forall isbyteZ (hmac256drbgabs_value state_abs)) &&
+                (hmac_drbg_update_post state_abs ctx info_contents
+                 * Stream s')
+          end
+        else
+          data_at Tsh t_struct_hmac256drbg_context_st
+        (md_ctx',
+        (map Vint (map Int.repr V),
+        (Vint (Int.repr reseed_counter),
+        (Vint (Int.repr entropy_len),
+        (Val.of_bool prediction_resistance, Vint (Int.repr reseed_interval))))))
+        ctx
+          * data_at Tsh t_struct_mbedtls_md_info info_contents (fst md_ctx')
+          * md_full md_ctx md_ctx'
+          * Stream s
+        ;
+        memory_block Tsh out_len output;
+      data_at Tsh (tarray tuchar add_len) (map Vint (map Int.repr contents))
+        additional;
+      spec_sha.K_vector kv)).
+  {
+    rename H10 into Hshould_reseed.
+    (* ret = mbedtls_hmac_drbg_reseed( ctx, additional, add_len ) *)
+    forward_call (contents, additional, add_len, ctx,
+                  (md_ctx',
+           (map Vint (map Int.repr V),
+           (Vint (Int.repr reseed_counter),
+           (Vint (Int.repr entropy_len),
+           (Val.of_bool prediction_resistance,
+           Vint (Int.repr reseed_interval)))))),
+                  (HMAC256DRBGabs md_ctx V reseed_counter entropy_len prediction_resistance reseed_interval),
+                  kv, info_contents, s).
+    {
+      unfold hmac256drbg_relate.
+      entailer!.
+    }
+    {
+      (* prove the PROP clauses *)
+      change (Int.max_unsigned) with 4294967295.
+      repeat split; auto; omega.
+    }
+    Intros vret; destruct vret as [state_abs return_value].
+    unfold hmac_drbg_update_post. Intros state.
+    forward.
+
+    forward_if (PROP  (return_value = Vzero)
+      LOCAL  (temp _ret return_value;
+      temp 158%positive (snd (state_abs, return_value)); 
+      temp _md_len md_len; temp _info (let (x, _) := md_ctx' in x);
+      temp _reseed_interval (Vint (Int.repr reseed_interval));
+      temp _reseed_counter (Vint (Int.repr reseed_counter));
+      temp _prediction_resistance (Val.of_bool prediction_resistance);
+      temp _out output; temp _left (Vint (Int.repr out_len)); 
+      temp _ctx ctx; temp _p_rng ctx; temp _output output;
+      temp _out_len (Vint (Int.repr out_len)); temp _additional additional;
+      temp _add_len (Vint (Int.repr add_len)); gvar sha._K256 kv;
+      temp 159%positive (Val.of_bool should_reseed))
+      SEP 
+      (hmac_drbg_update_post (fst (state_abs, return_value)) ctx
+         info_contents;
+      data_at Tsh (tarray tuchar add_len) (map Vint (map Int.repr contents))
+        additional;
+      Stream
+        (get_stream_result
+           (mbedtls_HMAC256_DRBG_reseed_function s
+              (HMAC256DRBGabs md_ctx V reseed_counter entropy_len
+                 prediction_resistance reseed_interval) contents));
+      K_vector kv; memory_block Tsh out_len output)).
+    {
+      (* return_value != 0 *)
+      forward.
+
+      rename H10 into Hreseed_result; simpl in Hreseed_result.
+      rename H11 into Hreturn_value; simpl in Hreturn_value.
+      assert (Hret_not_0: _id0 <> Int.zero).
+      {
+        clear - H14.
+        intros contra. subst.
+        inversion H14.
+      }
+      destruct state_abs.
+      destruct state as [md_ctx0' [V' [reseed_counter' [entropy_len' [prediction_resistance' reseed_interval']]]]].
+
+      unfold hmac_drbg_update_post, get_stream_result, hmac256drbg_relate.
+      Exists (HMAC256DRBGabs md_ctx V reseed_counter entropy_len prediction_resistance reseed_interval) (Vint _id0) (md_ctx0',
+        (map Vint (map Int.repr V),
+        (Vint (Int.repr reseed_counter),
+        (Vint (Int.repr entropy_len),
+        (Val.of_bool prediction_resistance, Vint (Int.repr reseed_interval)))))).
+      apply orb_true_iff in Hshould_reseed.
+      replace (Z.of_nat (length contents)) with (Zlength contents) by (rewrite Zlength_correct; auto).
+      rewrite Hout_lenb in *. rewrite Hadd_lenb in *.
+      rewrite andb_negb_r in *.
+      destruct md_ctx.
+      remember (get_entropy 256 entropy_len entropy_len prediction_resistance s) as get_entropy_result; destruct get_entropy_result.
+      {
+        (* entropy succeeded - not possible *)
+        clear - Hreturn_value Hret_not_0.
+        unfold return_value_relate_result in Hreturn_value.
+        idtac.
+        inv Hreturn_value.
+        assert (contra: False) by (apply Hret_not_0; auto); inversion contra.
+      }
+      (* entropy failed *)
+      unfold hmac256drbgabs_relate_reseed_result in Hreseed_result.
+      inv Hreseed_result.
+      destruct Hshould_reseed as [Hpr | Hcount].
+      {
+        (* prediction_resistance = true *)
+        subst.
+        entailer!.
+      }
+      {
+        (* reseed_counter > reseed_interval *)
+        destruct prediction_resistance0; [entailer!|].
+        unfold HMAC256_DRBG_generate_algorithm.
+        unfold HMAC_DRBG_generate_algorithm.
+        rename H4 into Hreseed_interval.
+        simpl in Hreseed_interval.
+        subst reseed_interval0.
+        rewrite Hcount.
+        unfold HMAC256_DRBG_reseed_function.
+        unfold DRBG_reseed_function.DRBG_reseed_function.
+        rewrite Hadd_lenb.
+        rewrite andb_negb_r.
+        rewrite <- Heqget_entropy_result.
+        entailer!.
+      }
+    }
+    {
+      (* return value = 0 *)
+      forward.
+
+      assert (Hret_eq_0: return_value = Vzero).
+      {
+        clear - H14.
+        destruct return_value; inv H14.
+        remember (Int.eq i (Int.repr 0)) as i_0; destruct i_0; inv H0.
+        apply binop_lemmas2.int_eq_true in Heqi_0.
+        rewrite Heqi_0; reflexivity.
+      }
+      subst return_value.
+      unfold hmac_drbg_update_post.
+      Exists state.
+      entailer!.
+    }
+
+    (* add_len = 0; *)
+    forward.
+
+    (* prove post condition of if statement *)
+    rename H10 into Hreseed_result.
+    rename H11 into Hreturn_value.
+    subst return_value.
+    destruct (mbedtls_HMAC256_DRBG_reseed_function s
+             (HMAC256DRBGabs md_ctx V reseed_counter entropy_len
+                prediction_resistance reseed_interval) contents); simpl in Hreturn_value.
+    Focus 2. destruct e; [inversion Hreturn_value | assert (contra: False) by (apply Hreturn_value; reflexivity); inversion contra].
+    destruct state_abs. destruct md_ctx0.
+    subst should_reseed. rewrite Hshould_reseed.
+    unfold hmac256drbgabs_convert_state_handle.
+    unfold hmac256drbgabs_relate_reseed_result in Hreseed_result.
+    destruct d as [[[[V1 key1] reseed_counter1] security_strength1] prediction_resistance1].
+    simpl in Hreseed_result.
+    destruct Hreseed_result as [Hkey1 [HV1 [Hreseed_counter1 [Hentropy_len [Hprediction_resistance1 Hreseed_interval1]]]]].
+    subst.
+    Exists data.
+    entailer!.
+  }
+  {
+    forward.
+
+    rewrite H10.
+    entailer!.
+  }
+
+  remember (if should_reseed then 0 else add_len) as add_len_new.
+
+  remember (if eq_dec additional nullval then false else if eq_dec add_len_new 0 then false else true) as non_empty_additional.
